translator/okasaki-examples/LazyPairingHeapScript.sml
@@ -23,8 +23,8 @@ val heap_to_bag_def = Define `
   BAG_INSERT x (BAG_UNION (heap_to_bag h1) (heap_to_bag h2)))`;
 
 val is_heap_ordered_def = Define `
-(is_heap_ordered get_key leq Empty = T) ∧
-(is_heap_ordered get_key leq (Tree x h1 h2) =
+(is_heap_ordered get_key leq Empty <=> T) ∧
+(is_heap_ordered get_key leq (Tree x h1 h2) <=>
   is_heap_ordered get_key leq h1 ∧
   is_heap_ordered get_key leq h2 ∧
   BAG_EVERY (\y. leq (get_key x) (get_key y)) (heap_to_bag h1) ∧
@@ -100,8 +100,8 @@ full_simp_tac (srw_ss()++numSimps.ARITH_AC_ss) [heap_size_def, merge_def] >>
 full_simp_tac (srw_ss()++ARITH_ss) []);
 
 val merge_size_lem = Q.prove (
-`heap_size (\x.0) (merge get_key leq (Tree x h1 h2) h1') <
-  heap_size (\x.0) h1 + heap_size (\x.0) h2 + heap_size (\x.0) h1' + 2 = T`,
+`(heap_size (\x.0) (merge get_key leq (Tree x h1 h2) h1') <
+  heap_size (\x.0) h1 + heap_size (\x.0) h2 + heap_size (\x.0) h1' + 2) = T`,
 rw [merge_size, heap_size_def] >>
 decide_tac);
 
